\documentclass{amsart}
%\usepackage{}
\renewcommand{\baselinestretch}{1.5}
\addtolength{\textwidth}{.2in}
\input{./my_latex_definitions.tex}

\begin{document}
\thispagestyle{empty}

\centerline{\Large Activity 11 -- Introduction to Proof}
\centerline{\large logical equivalence}

\bigskip
\Large

It may be useful to have a copy of the table of basic logical equivalences handy while working on these.  In addition to the equivalences in the table, recall the following:

$A \iff B \; \cong \; (A \implies B) \land (B \implies A)$ 

and $A \implies B \; \cong \; \lnot A \lor B$.

\vspace{.2in}

\begin{enumerate}

\item Fill in the right-hand column with explanations for each step in the following two column proof.

We want to show that $(A \lor \lnot B) \land (B \lor \lnot A)$ is logically equivalent to $(A \land B) \lor (\lnot B \land \lnot A)$.

\vspace{.5in}

\hspace{-1in} \begin{tabular}{c | c}
$(A \lor \lnot B) \land (B \lor \lnot A)$ & \rule{2.5in}{0in} \\
\rule{0pt}{18pt} & \\
$((A \lor \lnot B) \land B) \lor (A \lor \lnot B) \land \lnot A)$ & \\
\rule{0pt}{18pt} & \\
$((A \land B) \lor (\lnot B \land B) ) \lor (A \lor \lnot B) \land \lnot A)$ & \\
\rule{0pt}{18pt} & \\
$((A \land B) \lor (\lnot B \land B) ) \lor ((A \land \lnot A) \lor (\lnot B \land \lnot A)) $ & \\
\rule{0pt}{18pt} & \\
$((A \land B) \lor c ) \lor (c \lor (\lnot B \land \lnot A)) $ & \\
\rule{0pt}{18pt} & \\
$(A \land B)  \lor (\lnot B \land \lnot A) $ & \\
\end{tabular}

\vspace{.5in}

\newpage

\item Fill in the rest of the left-hand column with logical expressions in the following two column proof.

We want to show that $ A \lor ({\lnot}A \land B) \; \cong \; A \lor B $.
\vspace{.5in}

\hspace{-1in} \begin{tabular}{c | c}
\rule{2.5in}{0in} & \rule{2.5in}{0in} \\
 $ A \lor ({\lnot}A \land B)$ & Given \\
\rule{0pt}{18pt} & \\
 & Distributive law \\
\rule{0pt}{18pt} & \\
 & Complementarity \\
\rule{0pt}{18pt} & \\
 & Identity law
\end{tabular}

\vspace{.75in}

\item Create two column proofs for the following:

\begin{enumerate}
\item \rule[-8pt]{0pt}{36pt} $((A \land B) \lor  (\lnot A \land B)  ) \land (A \land B) \; \cong \; A \land B $
\item \rule[-8pt]{0pt}{36pt} $A \; \cong \; A \land ((A \lor {\lnot}B) \lor (A \lor B))$
\item \rule[-8pt]{0pt}{36pt} ${\lnot}(A \land B) \land {\lnot}(A \land C) \; \cong \; {\lnot}A \lor ({\lnot}B \land {\lnot}C)$
\item \rule[-8pt]{0pt}{36pt} $ A \iff B \; \cong \; (A \land B) \lor (\lnot A \land \lnot B)$
\end{enumerate}
 
\end{enumerate}

\end{document}
