Write two-column proofs that verify each of the following
logical equivalences.

\begin{enumerate}
\item $A \lor (A \land B) \; \cong \; A \land (A \lor B)$
\medskip

\item $(A \land {\lnot}B) \lor A \; \cong \; A$
\medskip

\item $A \lor B \; \cong \; A \lor ({\lnot}A \land B)$
\medskip

\item ${\lnot}(A \lor {\lnot}B) \lor ({\lnot}A \land {\lnot}B) \; \cong \; {\lnot}A$
\medskip

\item $A \; \cong \; A \land ((A \lor {\lnot}B) \lor (A \lor B))$
\medskip

\item $(A \land {\lnot}B) \land ({\lnot}A \lor B) \; \cong \; c$
\medskip

\item $A \; \cong \; A \land (A \lor (A \land (B \lor C)))$
\medskip

\item ${\lnot}(A \land B) \land {\lnot}(A \land C) \; \cong \; {\lnot}A \lor ({\lnot}B \land {\lnot}C)$
\medskip

\end{enumerate}

\hint{
Here's the last one:

\begin{proof}

$  {\lnot}(A \land B) \land {\lnot}(A \land C) $ \\  
 \rule{0pt}{0pt} \hfill \parbox{3in}{\color[rgb]{1,0,0}  	 DeMorgan's law (times 2)} \\
$\equiv  \quad   ({\lnot}A \lor {\lnot}B) \land ({\lnot}A \lor {\lnot}C)	$ \\   
 \rule{0pt}{0pt} \hfill \parbox{3in}{\color[rgb]{1,0,0}  	 Distributive law} \\ 
$\equiv  \quad  {\lnot}A \lor ({\lnot}B \land {\lnot}C) $ \\  
\end{proof}

}
\workbookpagebreak

\rule{0pt}{0pt}

\workbookpagebreak